poly-reductions-master/Cook_Levin/Complexity_classes/Bit_Length.thy
@@ -1,7 +1,0 @@
-theory Bit_Length
-  imports Main "HOL-Library.Discrete"
-begin
-
-definition bit_length :: "nat \<Rightarrow> nat" where 
-"bit_length = Discrete.log"
-end
