turing_to_while/tape_nat_conversion.thy
@@ -1,0 +1,152 @@
+theory tape_nat_conversion
+  imports Main "Turing" "../IMP-/Com" "../IMP-/Big_StepT" "../IMP-/Small_StepT" "../IMP-/Big_Step_Small_Step_Equivalence"  "../IMP-/Max_Constant"
+begin
+
+text "In this theory we prove the conversion between natural numbers and the tape as described in turing.thy . 
+Note that this closely mirrors the conversion between a binary (in string format or similar) and natural numbers"
+type_synonym enc_tape = "nat \<times> nat \<times> nat"
+abbreviation LeftShift_nat:: "nat \<Rightarrow> nat" where
+" LeftShift_nat a \<equiv> a + a"
+
+subsection "Conversion from tape to natural"
+fun tape_to_nat :: "cell list \<Rightarrow> nat" where
+"tape_to_nat [] = 0" |                
+"tape_to_nat (x#xs) = (if x = Bk then LeftShift_nat (tape_to_nat xs)
+                                   else LeftShift_nat (tape_to_nat xs) + 1)"
+
+fun encode_tape :: "config \<Rightarrow> enc_tape" where
+"encode_tape (s,ls,rs) = (s, tape_to_nat ls, tape_to_nat rs)"
+
+lemma t2n_0: "(\<forall>x\<in> set xs. x = Bk) \<longleftrightarrow>  tape_to_nat xs = 0 "
+  apply(induct xs)
+   apply(auto)
+  done
+
+lemma tape_to_nat_even: "even (tape_to_nat xs) \<longleftrightarrow> hd xs = Bk \<or> xs = []"
+  apply (induct xs)
+   apply(auto)
+  done
+
+lemma tape_to_nat_odd: " xs \<noteq> [] \<Longrightarrow> odd (tape_to_nat xs) \<longleftrightarrow> hd xs = Oc"
+  apply (induct xs)
+  using cell.exhaust by auto
+
+subsection "Conversion from natural to tape"
+fun nat_to_tape :: "nat \<Rightarrow> cell list" where
+"nat_to_tape 0 = []" |
+"nat_to_tape n = (if (n mod 2) = 1 then Oc else Bk) # nat_to_tape (n div 2)"
+
+
+fun decode_tape :: "enc_tape \<Rightarrow> config" where
+"decode_tape (z,n,m) = (z, nat_to_tape n, nat_to_tape m)"
+
+lemma nat_to_tape_double[simp]: "n > 0 \<Longrightarrow> nat_to_tape (2 * n) = Bk # (nat_to_tape n)"
+  apply(induct n)
+   apply(auto)
+  done
+
+lemma nat_to_tape_nth_bit: "nat_to_tape (2^n) = replicate n Bk  @ [Oc]"
+  apply(induct n)
+   apply(auto)
+  done
+
+
+text "This function is used to compare tapes with each other. Two tapes are considered equal, 
+if they are the same ignoring any leading blank cells."
+fun is_cell_list_eq :: "cell list \<Rightarrow> cell list \<Rightarrow> bool" where 
+"is_cell_list_eq xs ys = (dropWhile (\<lambda>x. x = Bk)(rev xs)  = dropWhile (\<lambda>y. y = Bk) (rev ys))"
+
+
+lemma tape_to_nat_app_bk[simp]: "tape_to_nat (xs @ [Bk]) = tape_to_nat xs"
+  apply(induct xs)
+   apply(auto)
+  done
+
+lemma is_cell_list_eq_same[simp]: "is_cell_list_eq xs xs"
+  apply(induct xs)
+   apply(auto)
+  done
+
+lemma is_cell_list_eq_com: "is_cell_list_eq xs ys \<Longrightarrow> is_cell_list_eq ys xs"
+  apply(induct xs)
+   apply(auto)
+  done
+
+lemma is_cell_list_eq_cons:
+  assumes "is_cell_list_eq xs ys"
+  shows "is_cell_list_eq (x#xs) (x#ys)"
+using assms proof -
+  have "(dropWhile (\<lambda>x. x = Bk)(rev xs) = dropWhile (\<lambda>y. y = Bk) (rev ys))" using assms by auto
+  then have "(if (\<forall>x\<in>set xs.  x = Bk) then dropWhile(\<lambda>x. x = Bk) [] else dropWhile (\<lambda>x. x = Bk) (rev xs) @ []) = 
+            (if (\<forall>x\<in>set ys.  x = Bk) then dropWhile(\<lambda>x. x = Bk) [] else dropWhile (\<lambda>x. x = Bk) (rev ys) @ [])" 
+    by (smt (verit, best) dropWhile_eq_Nil_conv set_rev)
+  then have "(if (\<forall>x\<in>set xs.  x = Bk) then dropWhile(\<lambda>x. x = Bk) [x] else dropWhile (\<lambda>x. x = Bk) (rev xs) @ [x]) = 
+            (if (\<forall>x\<in>set ys.  x = Bk) then dropWhile(\<lambda>x. x = Bk) [x] else dropWhile (\<lambda>x. x = Bk) (rev ys) @ [x])"
+    by (smt (verit, best) \<open>dropWhile (\<lambda>x. x = Bk) (rev xs) = dropWhile (\<lambda>y. y = Bk) (rev ys)\<close> dropWhile_eq_Nil_conv set_rev)
+  then have "(dropWhile (\<lambda>x. x = Bk)((rev xs) @ [x]) = dropWhile (\<lambda>y. y = Bk) ((rev ys) @ [x]))" by (simp add: dropWhile_append)
+  then show ?thesis by simp
+qed
+
+
+lemma tape_to_nat_inverse: "tape_to_nat(nat_to_tape n) = n"
+proof(induct n rule: nat_to_tape.induct)
+  case 1
+  then show ?case by simp
+next
+  case (2 v)
+  then show ?case
+    proof (cases v rule: parity_cases)
+    case even
+    then have "tape_to_nat (nat_to_tape (Suc v)) = tape_to_nat (Oc # nat_to_tape (Suc v div 2))" by auto
+    also have "... = 2 * tape_to_nat(nat_to_tape (Suc v div 2)) + 1" by simp
+    also have "... = 2 * (Suc v div 2) + 1" using "2" by simp
+    then show ?thesis by (metis calculation even(1) even_Suc odd_two_times_div_two_succ)
+  next
+    case odd
+    then have "tape_to_nat (nat_to_tape (Suc v)) = tape_to_nat (Bk # nat_to_tape (Suc v div 2))" by simp
+    also have "... = 2 * tape_to_nat (nat_to_tape (Suc v div 2))" by simp
+    also have "... = 2 * Suc v div 2" by (metis "2" div_mult_swap even_Suc odd(1))
+    finally show ?thesis by auto
+        qed
+qed
+
+lemma nat_to_tape_inverse: "is_cell_list_eq (nat_to_tape(tape_to_nat xs)) xs"
+proof (induction xs rule: tape_to_nat.induct)
+  case 1
+  then show ?case by simp
+next
+  case (2 x xs)
+  then show ?case proof (cases x)
+    case Bk
+    then have "is_cell_list_eq (nat_to_tape(tape_to_nat xs)) xs" using 2 by simp
+    then have Bk_cons: "is_cell_list_eq (Bk # nat_to_tape(tape_to_nat xs)) (Bk#xs)" using is_cell_list_eq_cons by fast
+    consider "(\<forall>x\<in>set xs. x = Bk)" | "Oc \<in> set xs" using cell.exhaust by auto
+    then have "is_cell_list_eq (nat_to_tape(2 * tape_to_nat xs)) (Bk#xs)" proof (cases)
+      case 1
+       then show ?thesis using t2n_0 Bk_cons by simp
+    next
+      case 2
+      then show ?thesis using Bk_cons using t2n_0 by fastforce
+    qed (* case distinction on xs all blank vs some Oc *)
+    then show ?thesis by (simp add: Bk mult_2)
+  next
+    case Oc
+    then have "is_cell_list_eq (nat_to_tape(tape_to_nat xs)) xs" using 2 by simp
+    then have "is_cell_list_eq (Oc # nat_to_tape(tape_to_nat xs)) (Oc#xs)" using is_cell_list_eq_cons by fast
+    then have "is_cell_list_eq (nat_to_tape(2 * tape_to_nat xs + 1)) (Oc#xs)" by simp
+    then show ?thesis by (simp add: Oc mult_2)
+  qed
+qed
+
+
+lemma encode_decode_inverse: "(z,x,y) = encode_tape(decode_tape(z,x,y))"
+  by (simp add: tape_to_nat_inverse)
+lemma decode_encode_inverse: 
+  assumes encoded_decoded: "(z1,x1,y1) = decode_tape(encode_tape(z,x,y))"
+  shows "z=z1 \<and> is_cell_list_eq x x1 \<and> is_cell_list_eq y y1"
+  using encoded_decoded nat_to_tape_inverse by auto
+
+
+
+
+end
